axioms.v
@@ -1,0 +1,113 @@
+(** * General Header Autosubst - Assumptions and Definitions *)
+
+(** ** Axiomatic Assumptions
+    For our development, during rewriting of the reduction rules,  we have to extend Coq with two well known axiomatic assumptions, namely _functional extensionality_ and _propositional extensionality_. The latter entails _proof irrelevance_.
+*)
+
+(** *** Functional Extensionality
+    We import the axiom from the Coq Standard Library and derive a utility tactic to make the assumption practically usable.
+*)
+Require Import Coq.Logic.FunctionalExtensionality.
+Require Import Program.Tactics.
+
+Tactic Notation "nointr" tactic(t) :=
+  let m := fresh "marker" in
+  pose (m := tt);
+  t; revert_until m; clear m.
+
+Ltac fext := nointr repeat (
+  match goal with
+    [ |- ?x = ?y ] =>
+    (refine (@functional_extensionality_dep _ _ _ _ _) ||
+     refine (@forall_extensionality _ _ _ _) ||
+     refine (@forall_extensionalityP _ _ _ _) ||
+     refine (@forall_extensionalityS _ _ _ _)); intro
+  end).
+
+
+(** ** Functor Instances
+
+Exemplary functor instances needed to make Autosubst's generation possible for functors.
+Two things are important:
+1. The names are fixed.
+2. For Coq to check termination, also the proofs have to be closed with Defined.
+ *)
+
+(** *** List Instance *)
+Require Export List.
+
+Definition funcomp {X Y Z} (g : Y -> Z) (f : X -> Y)  :=
+  fun x => g (f x).
+
+Notation "'list_map'" := map.
+
+Definition list_ext {A B} {f g : A -> B} :
+  (forall x, f x = g x) -> forall xs,  list_map f xs = map g xs.
+  intros H. induction xs. reflexivity.
+  cbn. f_equal. apply H. apply IHxs.
+Defined.
+
+Definition list_id {A}  { f : A -> A} :
+  (forall x, f x = x) -> forall xs, List.map f xs = xs.
+Proof.
+  intros H. induction xs. reflexivity.
+  cbn. rewrite H. rewrite IHxs; eauto.
+Defined.
+
+Definition list_comp {A B C} {f: A -> B} {g: B -> C} {h} :
+  (forall x, (funcomp  g f) x = h x) -> forall xs, map g (map f xs) = map h xs.
+Proof.
+  induction xs. reflexivity.
+  cbn. rewrite <- H. f_equal. apply IHxs.
+Defined.
+
+(** *** Prod Instance *)
+
+Definition prod_map {A B C D} (f : A -> C) (g : B -> D) (p : A * B) :
+  C * D.
+Proof.
+  destruct p. split. auto. auto.
+Defined.
+
+Definition prod_id {A B} {f : A -> A} {g : B -> B} :
+  (forall x, f x = x) -> (forall x, g x = x) -> forall p, prod_map f g p = p.
+Proof.
+  intros. destruct p. cbn. f_equal; auto.
+Defined.
+
+Definition prod_ext {A B C D} {f f' : A -> C} {g g': B -> D} :
+  (forall x, f x = f' x) -> (forall x, g x = g' x) -> forall p, prod_map f g p = prod_map f' g' p.
+Proof.
+  intros. destruct p. cbn. f_equal; auto.
+Defined.
+
+Definition prod_comp {A B C D E F} {f1 : A -> C} {g1 : C -> E} { h1} {f2: B -> D} {g2: D -> F} {h2}:
+  (forall x, (funcomp  g1 f1) x = h1 x) -> (forall x, (funcomp g2 f2) x = h2 x) -> forall p, prod_map g1 g2 (prod_map f1 f2 p) = prod_map h1 h2 p.
+Proof.
+  intros. destruct p. cbn. f_equal; auto.
+  now rewrite <- H. now rewrite <- H0.
+Defined.
+
+
+(** *** Function Instance *)
+
+Definition cod X A:  Type :=  X -> A.
+
+Definition cod_map {X} {A B} (f : A -> B) (p : X -> A) :
+  X -> B.
+Proof. eauto. Defined.
+
+(** Note that this requires functional extensionality. *)
+Definition cod_id {X} {A} {f : A -> A} :
+  (forall x, f x = x) -> forall (p: X -> A), cod_map f p = p.
+Proof. intros H p. unfold cod_map. fext. congruence. Defined.
+
+Definition cod_ext {X} {A B} {f f' : A -> B} :
+  (forall x, f x = f' x) -> forall (p: X -> A), cod_map f p = cod_map f' p.
+Proof. intros H p. unfold cod_map. fext. congruence. Defined.
+
+Definition cod_comp {X} {A B C} {f : A -> B} {g : B -> C} {h} :
+  (forall x, (funcomp g f) x =  h x) -> forall (p: X -> _), cod_map g (cod_map f p) = cod_map h p.
+Proof. intros H p. unfold cod_map. fext. intros x. now rewrite <- H. Defined.
+
+Hint Rewrite in_map_iff : FunctorInstances.
